Arithmetization/ISigmaOne/HFS/Seq.lean
@@ -376,7 +376,7 @@ lemma mkSeq₂_defined : 𝚺₁-Function₂ (fun x y : V ↦ !⟦x, y⟧) via m
 
 instance mkSeq₂_definable : 𝚺₁-Function₂ (fun x y : V ↦ !⟦x, y⟧) := mkSeq₂_defined.to_definable
 
-instance mkSeq₂_definable' (Γ m) : Γ-[m + 1]-Function₂ (fun x y : V ↦ !⟦x, y⟧) := .of_sigmaOne mkSeq₂_definable _ _
+instance mkSeq₂_definable' (Γ m) : Γ-[m + 1]-Function₂ (fun x y : V ↦ !⟦x, y⟧) := mkSeq₂_definable.of_sigmaOne
 
 end
 
